<?xml version='1.0' encoding="utf-8"?>
<!--
% !TEX TS-program = PreTeXt-HTML
-->
<section xml:id="week-4" xmlns:xi="http://www.w3.org/2001/XInclude">
			<title>Week 4</title>
			<exercise>
			 	<title>Infinite series</title>
				<task>
					<statement>
					Given a sequence of real numbers, define the corresponding <em><m>N</m>th partial sum</em> and <em>infinite series</em>. When do we say the infinite series <em>exists</em>? What is a <em>term</em> of an infinite series?
					</statement>
					<solution>
						<definition>
							<title>Infinite series</title>
							<statement>
Given a sequence of real numbers <m>(a_n)_{n=1}^\infty</m> and <m>N\in \N</m>, the <em><m>N</m>th partial sum</em> is given by
<me>
\sum_{n=1}^N a_n := a_1 + a_2 + \dots + a_N.
</me>
If the sequence of partial sums tends to a limit as <m>N \to \infty</m>, then the corresponding  <em>infinite series</em> exists and is equal to the limit
<me>
 \lim_{N\to\infty} \sum_{n=1}^Na_n, \quad \text{written}\quad \sum_{n=1}^\infty a_n.
</me>
The <em>terms</em> of the infinite series <m>\displaystyle \sum_{n=1}^\infty a_n</m> are the summands <m>a_n</m>.
</statement>
</definition>
					</solution>
				</task>
				<task>
					<statement>
					Justify why an infinite series always exists when the terms are non-negative.
					</statement>
					<solution>
					<remark xml:id="rem-non-neg-seq">
 Suppose that the sequence <m>(a_n)_{n=1}^\infty</m> is non-negative, so that <m>a_n \geq 0</m> for all <m>n\in \N</m>.
 Then the sequence of partial sums 
<me>
a_1 \quad \leq\quad a_1 + a_2 \quad \leq\quad a_1 + a_2 + a_3 \quad \leq\quad \dots 
</me>
is an increasing sequence of real numbers.
 Hence by the monotone convergence principle (<xref ref="prop-mono-lim"/>), the limit
<me>
\sum_{n=1}^\infty a_n = \lim_{N\to \infty} \sum_{n=1}^Na_n
</me>
always exists, but is possibly <m>\infty</m>.
 We write
<me>
\sum_{n=1}^\infty a_n \lt  \infty
</me>
to indicate that the series converges to a real number (when the underlying sequence <m>(a_n)</m> is non-negative).
</remark>
					</solution>
				</task>
				<task>
					<statement>
					Define what it means for an infinite series to be <em>convergent</em>. Give both an example and non-example, with proof.
					</statement>
					<solution>
					Let <m>(a_n)_{n=1}^\infty</m> be a sequence of real numbers. If the limit  <m>\displaystyle\sum_{n=1}^\infty a_n=\lim_{N\to \infty} \sum_{n=1}^N a_n</m> exists and equals a <em>finite real number</em>, then we say that the series <m>\displaystyle\sum_{n=1}^\infty a_n </m> is <em>convergent</em>.	
					</solution>
				</task>
				<task>
					<statement>
					Define what it means for an infinite series to be <em>absolutely convergent</em>. Given both an example and a non-example, with proof.
					</statement>
					<solution>
					We say that the series <m>\displaystyle\sum_{n=1}^\infty a_n</m> is <em>absolutely convergent</em> if
<me>
\sum_{n=1}^\infty |a_n| \lt  \infty.
</me>
 We say that the series is <em>conditionally covergent</em> if it is convergent but not absolutely convergent.
					</solution>
				</task>
				<task>
					<statement>State and prove the value of the <em>geometric series</em>.</statement>
					<solution>
						<example xml:id="eg-geo-series">
							<title>Geometric series</title>
							If <m>|x|\lt 1</m>, then
							<me>
\sum_{n=0}^\infty x^n = \frac{1}{1-x}.
</me>
				<proof>			
We have 
<me> \sum_{n=0}^N x^n  = 1 + \brac{x\sum_{n=0}^{N-1} x^n}  =  1+ \brac{x\sum_{n=0}^N x^n}- x^{N+1} .</me>
 Re-arranging (provided that <m>x \neq 1</m>) gives
<me>
\sum_{n=0}^N x^n = \frac{1-x^{N+1}}{1-x}.
</me>
 If <m>|x| \lt  1</m> then <m>x^N \to 0</m> as <m>N\to \infty</m>  by <xref ref="prop-geom-seq"/>.
 By the algebra of limits (<xref ref="prop-add-rule"/>, <xref ref="prop-mult-rule"/> and <xref ref="prop-recip-rule"/>) we have
<me>
\lim_{N \to \infty} \sum_{n=0}^N x^n = \lim_{N \to \infty} \frac{1-x^{N+1}}{1-x} = \frac{1 - x\displaystyle\lim_{N\to \infty} x^N}{1-x} = \frac{1}{1-x}.
</me>
</proof>
</example>
</solution>
				</task>
				<task>
					<statement>State and prove how infinite series respect both addition and scalar multiplication.
					</statement>
					<solution>
						<proposition xml:id="prop-lin-series">
							<title>Linearity of series</title>
							<statement>
 Suppose that the series <m>\displaystyle\sum_{n=1}^\infty a_n</m> and <m>\displaystyle\sum_{n=1}^\infty b_n</m> both converge. 
 Let <m>\lambda, \mu \in \R</m>.
 Then the  series <m>\displaystyle\sum_{n=1}^\infty (\lambda a_n + \mu b_n)</m> converges and satisfies the identity
<me>
\sum_{n=1}^\infty (\lambda a_n + \mu b_n) = \lambda \sum_{n=1}^\infty a_n + \mu \sum_{n=1}^\infty b_n.
</me>
</statement>
<proof>
This is an application of the addition and multiplication rules for sequences (<xref ref="prop-add-rule"/> and <xref ref="prop-mult-rule"/>), as follows:
<md>
<mrow>
\sum_{n=1}^\infty (\lambda a_n + \mu b_n) \amp = \lim_{N \to \infty} \sum_{n=1}^N (\lambda a_n + \mu b_n)\qquad \text{[definition of series]}
</mrow>
<mrow>
\amp = \lim_{N \to \infty}\brac{ \lambda {\sum_{n=1}^N a_n} + \mu{\sum_{n=1}^N b_n}}\qquad \text{[linearity of finite sums]}
</mrow>
<mrow>
\amp =  \lim_{N \to \infty}\brac{ \lambda\sum_{n=1}^N a_n} + \lim_{N \to \infty}\brac{\mu\sum_{n=1}^N b_n} \qquad \text{[addition rule]}
</mrow>
<mrow>
\amp = \lambda \lim_{N \to \infty}\sum_{n=1}^N a_n + \mu \lim_{N \to \infty}\sum_{n=1}^N b_n\qquad \text{[multiplication rule]}.
</mrow>
</md>
</proof>
</proposition>
					</solution>
				</task>
			</exercise>
			<exercise>
				<title>Tests for convergence</title>
				<task>
					<statement>State and prove how absolute convergence implies convergence, together with the "infinite triangle inequality".
					</statement>
					<solution>
						<proposition xml:id="prop-abs-conv">
							<title>Absolute convergence implies convergence</title>
							<statement>
							<p>
 Let <m>(a_n)_{n=1}^\infty</m> be a sequence of real numbers.  If
<m>\displaystyle
\sum_{n=1}^\infty |a_n| \lt  \infty
</m>
then the series 
<m>\displaystyle
\sum_{n=1}^\infty a_n
</m>
converges to a finite real number. 
</p>
<p>
In addition, we have the infinite triangle inequality
<men xml:id="item-inf-tri">
\abs{\sum_{n=1}^\infty a_n }\leq \sum_{n=1}^\infty |a_n|.
</men>
</p>
</statement>
<proof>
<p>
Recall that the limit <m>\sum_n |a_n|</m> always exists (but is possibly infinite), by the monotone convergence principle (<xref ref="prop-mono-lim"/>), as in <xref ref="rem-non-neg-seq"/>.
 To prove that the series <m>\sum_n a_n</m> converges, it suffices to prove that the sequence of partial sums <m>\sum_{n=1}^N a_n</m> is a Cauchy sequence (<xref ref="def-cauchy"/>), since Cauchy sequences converge (<xref ref="prop-cauchy"/>).
 To this end, let <m>\eps \gt 0</m>. Since we are assuming that <m>\sum_{n=1}^N |a_n|</m> tends to a real limit as <m>N \to \infty</m>, we know that this is a Cauchy sequence (<xref ref="prop-cauchy"/>). 
 Hence there exists <m>N_0 \in \N</m> such that for all <m>M\gt N \geq N_0</m> we have
<me>
\eps \geq \abs{\sum_{n=1}^M |a_n| - \sum_{n=1}^N |a_n|} = \sum_{n=N+1}^M |a_n|.
</me>
 By the triangle inequality, for all <m>M \gt N \geq N_0</m> we have that
<me>
\abs{ \sum_{n=1}^M a_n - \sum_{n=1}^N a_n} = \abs{\sum_{n=N+1}^M a_n} \leq \sum_{n=N+1}^M |a_n| \leq \eps.
</me>
 This establishes the Cauchy property, as claimed.
 </p>
 <p>
 To prove the infinite triangle inequality <xref ref="item-inf-tri"/> we first observe the finite triangle inequality
<me>
-\sum_{n=1}^N |a_n| \leq \sum_{n=1}^N a_n \leq \sum_{n=1}^N |a_n|
</me>
 The infinite triangle inequality follows on letting <m>N \to \infty</m> and applying  the inequality rule for limits (<xref ref="prop-ineq-rule"/>) to either side of the above.
 </p>
 </proof>
 </proposition>
					</solution>
				</task>
				<task>
					<statement>State and prove the "<m>n</m>th term test" for non-convergence of infinite series.
					</statement>
					<solution>
						<proposition xml:id="prop-tail">
							<title><m>n</m>th term test</title>
							<statement>
 Suppose that the sequence <m>(a_n)_n</m> does not tend to zero, written <m>a_n \not\to 0</m> (or equivalently <m>|a_n| \not\to 0</m>). 
 Then the series <m>\displaystyle \sum_{n=1}^\infty a_n</m> does not converge.
 							</statement>
							<proof>
							We prove the <url href="https://en.wikipedia.org/wiki/Contraposition" visual="en.wikipedia.org/wiki/Contraposition">contrapositive</url>. To this end, suppose that <m>\displaystyle \sum_{n=1}^\infty a_n</m> converges to a real number.
 Then by <xref ref="prop-cauchy"/>, the sequence of partial sums
<me>
\brac{\sum_{n=1}^{N} a_n}_{N=1}^\infty
</me>
is a Cauchy sequence.
 Hence for any <m>\eps \gt 0</m> there exists <m>N_0 = N_0(\eps)</m> such that for all <m>N, M\geq N_0(\eps)</m> we have
<me>
\abs{\sum_{n=1}^M a_n - \sum_{n=1}^N a_n} \leq \eps.
</me>
 In particular, if <m>N-1 \geq N_0(\eps)</m> then we have
<me>
\abs{\sum_{n=1}^N a_n - \sum_{n=1}^{N-1} a_n}\leq \eps.
</me>
 It follows that <m>a_N \to 0</m> according to <xref ref="def-seq-limit"/>.
							</proof>
							</proposition>
 
					</solution>
				</task>
				<task>
					<statement>State and prove the "comparison test" for convergence of infinite series.
					</statement>
					<solution>
						<proposition xml:id="prop-oh-test">
							<title>Comparison test</title>
							<statement>
 Let <m>(a_n)_{n=1}^\infty</m> and <m>(b_n)_{n=1}^\infty</m> be sequences of real numbers.
 Suppose that <m>|a_n| \leq b_n</m> for all <m>n</m> and
 <me>
 \sum_{n=1}^\infty b_n  \lt  \infty.
</me>
 Then <m>\displaystyle \sum_{n=1}^\infty a_n</m> converges absolutely.
 							</statement>
							<proof>
							Notice that we must have <m>b_n \geq 0</m> for all <m>n</m>. Hence for any <m>N</m> we have
<me>
\sum_{n=1}^N |a_n| \leq \sum_{n=1}^N b_n \leq  \sum_{n=1}^\infty b_n.
</me>
 Therefore the sequence of partial sums <m>\displaystyle \sum_{n=1}^N |a_n|</m> is an increasing sequence bounded above by the real number
<m>\displaystyle  \sum_{n=1}^\infty b_n</m>. 
 Hence, by the monotone convergence principle (<xref ref="prop-mono-lim"/>), the sequence of partial sums <m>\displaystyle \sum_{n=1}^N |a_n|</m> converges to a real number.
 This proves absolute convergence (and hence convergence).
</proof>
</proposition>
					</solution>
				</task>
				<task>
					<statement>State and prove the "limit comparison test" for convergence of infinite series.
					</statement>
					<solution>
						<corollary>
							<title>Limit comparison test</title>
							<statement>
 Let <m>(a_n)_{n=1}^\infty</m> and <m>(b_n)_{n=1}^\infty</m> be sequences of real numbers with  <m>b_n \gt 0</m> positive for all <m>n</m>.
 Suppose that<fn>In particular, the limit exists.</fn>
<me>
\lim_{n\to \infty}\frac{|a_n|}{b_n} \lt  \infty \quad\text{and} \quad\sum_{n=1}^\infty b_n  \lt  \infty.
</me>
 Then <m>\displaystyle \sum_{n=1}^\infty a_n</m> converges absolutely.
</statement>
<proof>
 Since the sequence <m>\brac{a_n/b_n}_{n=1}^\infty</m> is convergent, it is bounded (<xref ref="prop-conv-bounded"/>).
 Hence there exists <m>M\gt 0</m> such that for all <m>n</m> we have 
 <m>
 |a_n|/b_n \leq M
 </m>, or equivalently 
  <me>
 |a_n| \leq Mb_n
 </me>. 
 By linearity of series (<xref ref="prop-lin-series"/>) we have
 <me>
 \sum_n(Mb_n) = M\sum_n b_n \lt \infty
 </me>.
 So the corollary follows from the comparison test (<xref ref="prop-oh-test"/>).
</proof>
</corollary>					</solution>
				</task>
				<task>
					<statement>State and prove the "ratio test" for convergence of infinite series.</statement>
					<solution>
					<corollary xml:id="cor-ratio">
					<title>Ratio test</title>
					<statement>
					<p>
 Let <m>(a_n)_{n=1}^\infty</m> be a sequence of <em>positive</em> real numbers.
 </p>
 <p>
 If 
<m>\displaystyle
\lim_{n\to \infty}\frac{a_{n+1}}{a_n} \lt  1 
</m>
 then 
<m>\displaystyle
\sum_{n=1}^\infty a_n \lt  \infty.
</m>
</p>
<p>
 If
<m>\displaystyle
\lim_{n\to \infty}\frac{a_{n+1}}{a_n} \gt 1 
</m> 
then 
<m>\displaystyle
\sum_{n=1}^\infty a_n =\infty.
</m>
</p>
</statement>
<proof>
<p>
 Write 
<me>
r:=\lim_{n\to \infty}\frac{a_{n+1}}{a_n}.
</me> 
 Let us first suppose that <m> r \lt  1</m>.
 Let <m>c</m> be a real number satisfying <m>r\lt  c \lt  1</m>, for instance <m>c := (r+1)/2</m>.
 Set 
<me>
\eps := c - r \gt 0.
</me>
 Then there exists <m>N</m> such that for <m>n \geq N</m> we have
<me>
\abs{\frac{a_{n+1}}{a_n}-  r}\leq \eps,
</me>
in particular
<me>
\frac{a_{n+1}}{a_n}\leq  r+  \eps = c.
</me>
 This implies that for <m>n \gt N</m> we have
<me>
a_{n} = a_{n-1} \frac{a_{n}}{a_{n-1}} \leq c a_{n-1}.
</me>
 Re-applying this argument, provided that <m>n-1 \gt N</m> we have
<me>
a_n \leq c^2 a_{n-2}.
</me>
 Iterating then gives that for <m>n \gt N</m> we have
<me>
a_n \leq c^{n-N} a_{N}
</me>
 Therefore, there exists a constant <m>M\gt0</m> such that for all <m>n</m> we have
<me>
a_n \leq Mc^n.
</me>
For instance, one could take 
<me>
M:=\max\set{a_1c^{-1},\dots, a_Nc^{-N}}
</me>.
 Since <m>c \lt  1</m>, we may sum the geometric series (<xref ref="eg-geo-series"/>) to deduce that <m>\sum_{n=1}^\infty Mc^n \lt  \infty</m>.
 Hence  the comparison test (<xref ref="prop-oh-test"/>) implies that <m>\sum_n a_n \lt  \infty</m>.
 </p>
 <p>
 Next suppose that the limit is <m>\gt 1</m>.
 Let <m>C</m> be a real number satisfying
<me>
1 \lt  C \lt  \lim_{n\to \infty}\frac{a_{n+1}}{a_n}.
</me>
 Then a similar argument to that given above yields <m>N \in \N</m> and <m>M\gt 0</m> such that
<me>
\frac{C^n}{M} \leq a_n  \quad \text{for all } n \geq N.
</me>
 Since <m>C \gt 1</m> the geometric series diverges <m>\sum_{n=N}^\infty M^{-1}C^n = \infty</m> (see <xref ref="eg-geo-series"/>), so the contrapositive of the comparison test (<xref ref="prop-oh-test"/>) implies that <m>\sum_{n=1}^\infty a_n = \infty</m>.
 </p>
</proof>
</corollary>
					</solution>
				</task>
				<task>
					<statement>State and prove the "alternating series test" for convergence of infinite series.</statement>
					<solution>
					<proposition xml:id="prop-alt-test">
						<title>Alternating series test</title>
						<statement>
 						Let <m>(a_n)_n</m> denote a <em>decreasing</em> sequence of <em>non-negative</em> reals, so that <m>a_n \geq a_{n+1} \geq 0</m> for all <m>n</m>. Suppose that <m>a_n \to 0</m>. Then the series
<me>
a_1-a_2+a_3-a_4 + \dots = \sum_{n=1}^\infty (-1)^{n+1} a_n 
</me>
converges.
						</statement>
					</proposition>
					Before proving the alternating series test, we prove the following key inequality.
					<lemma xml:id="lem-alt-ineq">
						<statement>
						For any decreasing sequence <m>b_1 \geq b_2 \geq \dots \geq b_n\geq 0</m> of non-negative reals, with finitely many terms, we have the inequalities
							<men xml:id="eq-alt-key-ineq">
							0 \leq b_1 - b_2 + \dots + (-1)^{n+1} b_n \leq b_1.
							</men>
						</statement>
						<proof>
						<title>Proof of <xref ref="lem-alt-ineq"/></title>
 We prove this by induction on <m>n</m>, the number of terms in the sequence.
 The basis case, when <m>n=1</m>, follows from the inequalities
<me>
0 \leq b_1 \leq b_1.
</me> 
 For the inductive step, we may suppose that
<me>
0 \leq b_2 -b_3 + \dots + (-1)^n b_{n} \leq b_2.
</me>
 It follows that
<me>
b_1 - b_2 + \dots + (-1)^{n+1} b_n = b_1- \brac{b_2 -b_3+ \dots + (-1)^{n} b_n} \geq b_1-b_2 \geq 0
</me>
and that
<me>
b_1 - b_2 + \dots + (-1)^{n+1} b_n = b_1- \brac{b_2 -b_3+ \dots + (-1)^{n} b_n} \leq b_1- 0= b_1.
</me>
</proof>
</lemma>
<proof>
<title>Proof of alternating series test (<xref ref="prop-alt-test"/>)</title>
 Applying the inequality <xref ref="eq-alt-key-ineq"/>, for any <m>N \gt M</m> we have
<md>
<mrow>
\abs{\sum_{n=1}^N(-1)^{n+1} a_n -\sum_{n=1}^M(-1)^{n+1} a_n } \amp= \abs{ \sum_{n=M+1}^N (-1)^{n+1} a_n}
</mrow>
<mrow>
 \amp = a_{M+1} - a_{M+2} + \dots + (-1)^{N-M+1} a_N
 </mrow>
<mrow>
 \amp \leq a_{M+1}.
 </mrow>
</md>
 Since <m>a_{n} \to 0</m> as <m>n \to \infty</m> there exists <m>N_0 = N_0(\eps)</m> such that for all <m>n \geq N_0(\eps)</m> we have <m>a_{n} \leq \eps</m>.
 In particular, if <m>N \gt M \geq N_0(\eps)</m> then 
<me>
\abs{\sum_{n=1}^N(-1)^{n+1} a_n -\sum_{n=1}^M(-1)^{n+1} a_n  }  \leq a_{M+1} \leq \eps.
</me>
 It follows that the sequence of partial sums
<me>
\sum_{n=1}^N (-1)^{n+1} a_n
</me>
is a Cauchy sequence (<xref ref="def-cauchy"/>), hence convergent (see <xref ref="prop-cauchy"/>).
</proof>
					</solution>
				</task>
				<task>
					<statement>State, but don't prove, the "integral estimate" (also known as the "integral test") for finite sums of decreasing sequences.</statement>
					<solution>
						<proposition xml:id="prop-int-test">
							<title>Integral test, proof deferred</title>
							<statement>
							Let <m>a,b \in \Z</m> with <m>a \lt  b</m>. Let <m>f : [a,b] \to \R</m> be a decreasing function<fn>Hence <em>Riemann integrable</em>, see ??.</fn>. Then
<men xml:id="prop-int-estimate">
f(a)+ \int_a^b f(t)\intd t \geq    \sum_{n=a}^b f(n) \geq f(b)+ \int_a^b f(t)\intd t.
</men>
							</statement>
						</proposition>
					</solution>
				</task>
			</exercise>
		</section>